Add new derived pattern and requirement on engine control program satisfying it

examples/Engine/P_2_Timeouts_Patterns.thy
@@ -1,21 +1,21 @@
 theory P_2_Timeouts_Patterns imports VCProving.Basic_Patterns 
 begin
 
-definition P_2_timeouts where "P_2_timeouts t1 t2 A1 A2 A3 A4 s \<equiv> (always (\<lambda> r2 r1 . ((weak_previous (\<lambda> r4 r3 . (\<not> (A1 r3))) r2 r1) \<or> ((since t1 A3 A2 r2 r1) \<or> (since t2 A4 True r2 r1)))) s)"
+definition P_release_2_timeouts where "P_release_2_timeouts t1 t2 A1 A2 A3 A4 A5 s \<equiv> (always (\<lambda> r2 r1 . ((weak_previous (\<lambda> r4 r3 . (\<not> (A1 r3))) r2 r1) \<or> ((since t1 A3 A2 r2 r1) \<or> ((since t2 A4 (\<lambda> r4 r3 . True) r2 r1) \<or> (A5 r2 r1))))) s)"
 
-definition P_2_timeouts_part where "P_2_timeouts_part t1 t2 A1 A2 A3 A4 s \<equiv> (P_2_timeouts t1 t2 A1 (\<lambda> s s1 . (A2 s1)) (\<lambda> s s1 . (A3 s1)) (\<lambda> s s1 . (A4 s1)) s)"
+definition P_release_2_timeouts_part where "P_release_2_timeouts_part t1 t2 A1 A2 A3 A4 A5 s \<equiv> (P_release_2_timeouts t1 t2 A1 (\<lambda> s s1 . (A2 s1)) (\<lambda> s s1 . (A3 s1)) (\<lambda> s s1 . (A4 s1)) (\<lambda> s s1 . (A5 s1)) s)"
 
-definition P_2_timeouts_inv where "P_2_timeouts_inv t1 t2 b_0 b_1 t1_0 b_2 t1_1 A1 A2_1 A3_1 A4_1 s \<equiv> ((((always_inv (\<lambda> r2 r1 . ((weak_previous (\<lambda> r4 r3 . (\<not> (A1 r3))) r2 r1) \<or> ((since t1 A3_1 A2_1 r2 r1) \<or> (since t2 A4_1 True r2 r1)))) s) \<and> (previous_inv b_0 (\<lambda> r4 r3 . (\<not> (A1 r3))) s)) \<and> (since_inv t1 b_1 t1_0 A3_1 A2_1 s)) \<and> (since_inv t2 b_2 t1_1 A4_1 True s))"
+definition P_release_2_timeouts_inv where "P_release_2_timeouts_inv t1 t2 b_0 b_1 t1_0 b_2 t1_1 A1 A2_1 A3_1 A4_1 A5_1 s \<equiv> ((((always_inv (\<lambda> r2 r1 . ((weak_previous (\<lambda> r4 r3 . (\<not> (A1 r3))) r2 r1) \<or> ((since t1 A3_1 A2_1 r2 r1) \<or> ((since t2 A4_1 (\<lambda> r4 r3 . True) r2 r1) \<or> (A5_1 r2 r1))))) s) \<and> (previous_inv b_0 (\<lambda> r4 r3 . (\<not> (A1 r3))) s)) \<and> (since_inv t1 b_1 t1_0 A3_1 A2_1 s)) \<and> (since_inv t2 b_2 t1_1 A4_1 (\<lambda> r4 r3 . True) s))"
 
-definition P_2_timeouts_inv_part where "P_2_timeouts_inv_part t1 t2 b_0 b_1 t1_0 b_2 t1_1 A1 A2 A3 A4 s \<equiv> (P_2_timeouts_inv t1 t2 b_0 b_1 t1_0 b_2 t1_1 A1 (\<lambda> s s1 . (A2 s1)) (\<lambda> s s1 . (A3 s1)) (\<lambda> s s1 . (A4 s1)) s)"
+definition P_release_2_timeouts_inv_part where "P_release_2_timeouts_inv_part t1 t2 b_0 b_1 t1_0 b_2 t1_1 A1 A2 A3 A4 A5 s \<equiv> (P_release_2_timeouts_inv t1 t2 b_0 b_1 t1_0 b_2 t1_1 A1 (\<lambda> s s1 . (A2 s1)) (\<lambda> s s1 . (A3 s1)) (\<lambda> s s1 . (A4 s1)) (\<lambda> s s1 . (A5 s1)) s)"
 
-lemma P_2_timeouts_inv_saving_gen: "
-P_2_timeouts_inv t1 t2 b_0 b_1 t1_0 b_2 t1_1 A1 A2_1 A3_1 A4_1 s0 \<Longrightarrow>
+lemma P_release_2_timeouts_inv_saving_gen: "
+P_release_2_timeouts_inv t1 t2 b_0 b_1 t1_0 b_2 t1_1 A1 A2_1 A3_1 A4_1 A5_1 s0 \<Longrightarrow>
 consecutive s0 s \<Longrightarrow>
-(((((True \<and> (((always_imp s0 (A3_1 s0) (A3_1 s)) \<and> (always_imp s0 (A2_1 s0) (A2_1 s))) \<and> ((always_imp s0 (A4_1 s0) (A4_1 s)) \<and> True))) \<and> (((b_0 s0) \<and> True) \<or> ((((t1 = 0) \<and> (A2_1 s s)) \<or> ((always_imp s0 (A3_1 s0) (A3_1 s)) \<and> ((always_imp s0 (A2_1 s0) (A2_1 s)) \<and> ((b_1 s) \<and> ((t1 <= ((t1_0 s0) + 1)) \<and> (A3_1 s s)))))) \<or> (((t2 = 0) \<and> True) \<or> ((always_imp s0 (A4_1 s0) (A4_1 s)) \<and> (True \<and> ((b_2 s) \<and> ((t2 <= ((t1_1 s0) + 1)) \<and> (A4_1 s s))))))))) \<and> ((b_0 s) --> (\<not> (A1 s)))) \<and> ((b_1 s) --> ((((t1_0 s) = 0) \<and> (A2_1 s s)) \<or> ((always_imp s0 (A3_1 s0) (A3_1 s)) \<and> ((always_imp s0 (A2_1 s0) (A2_1 s)) \<and> ((b_1 s) \<and> (((t1_0 s) <= ((t1_0 s0) + 1)) \<and> (A3_1 s s)))))))) \<and> ((b_2 s) --> ((((t1_1 s) = 0) \<and> True) \<or> ((always_imp s0 (A4_1 s0) (A4_1 s)) \<and> (True \<and> ((b_2 s) \<and> (((t1_1 s) <= ((t1_1 s0) + 1)) \<and> (A4_1 s s)))))))) \<Longrightarrow>
-P_2_timeouts_inv t1 t2 b_0 b_1 t1_0 b_2 t1_1 A1 A2_1 A3_1 A4_1 s"
+(((((True \<and> (((always_imp s0 (A3_1 s0) (A3_1 s)) \<and> (always_imp s0 (A2_1 s0) (A2_1 s))) \<and> (((always_imp s0 (A4_1 s0) (A4_1 s)) \<and> True) \<and> (always_imp s0 (\<lambda> r1 . (A5_1 s0 r1)) (\<lambda> r1 . (A5_1 s r1)))))) \<and> (((b_0 s0) \<and> True) \<or> ((((t1 = 0) \<and> (A2_1 s s)) \<or> ((always_imp s0 (A3_1 s0) (A3_1 s)) \<and> ((always_imp s0 (A2_1 s0) (A2_1 s)) \<and> ((b_1 s0) \<and> ((t1 <= ((t1_0 s0) + 1)) \<and> (A3_1 s s)))))) \<or> ((((t2 = 0) \<and> True) \<or> ((always_imp s0 (A4_1 s0) (A4_1 s)) \<and> (True \<and> ((b_2 s0) \<and> ((t2 <= ((t1_1 s0) + 1)) \<and> (A4_1 s s)))))) \<or> (A5_1 s s))))) \<and> ((b_0 s) --> (\<not> (A1 s)))) \<and> ((b_1 s) --> ((((t1_0 s) = 0) \<and> (A2_1 s s)) \<or> ((always_imp s0 (A3_1 s0) (A3_1 s)) \<and> ((always_imp s0 (A2_1 s0) (A2_1 s)) \<and> ((b_1 s0) \<and> (((t1_0 s) <= ((t1_0 s0) + 1)) \<and> (A3_1 s s)))))))) \<and> ((b_2 s) --> ((((t1_1 s) = 0) \<and> True) \<or> ((always_imp s0 (A4_1 s0) (A4_1 s)) \<and> (True \<and> ((b_2 s0) \<and> (((t1_1 s) <= ((t1_1 s0) + 1)) \<and> (A4_1 s s)))))))) \<Longrightarrow>
+P_release_2_timeouts_inv t1 t2 b_0 b_1 t1_0 b_2 t1_1 A1 A2_1 A3_1 A4_1 A5_1 s"
 
-unfolding P_2_timeouts_inv_def
+unfolding P_release_2_timeouts_inv_def
 apply(erule conjE)
 apply(erule conjE)
 subgoal premises prems1
@@ -64,15 +64,24 @@ apply(erule always_rule)
                 apply assumption
               done
           apply(insert prems6(1,3))
-            apply(rule since_L4)
+            apply(rule always_disj_rule)
             apply simp
               apply(erule conjE)
               subgoal premises prems8
               apply(rule conjI)
               apply(insert prems8(1,2))[1]
-                apply assumption
+                apply(rule since_L4)
+                apply simp
+                  apply(erule conjE)
+                  subgoal premises prems9
+                  apply(rule conjI)
+                  apply(insert prems9(1,2))[1]
+                    apply assumption
+                  apply(insert prems9(1,3))
+                    apply(rule always_imp_refl)
+                  done
               apply(insert prems8(1,3))
-                apply(rule always_imp_refl)
+                apply assumption
               done
           done
       done
@@ -82,11 +91,11 @@ apply(erule always_rule)
       apply(rule weak_previous_one_point[OF prems3(3)])
       apply simp
         apply(erule conjE)
-        subgoal premises prems9
+        subgoal premises prems10
         apply(rule conjI)
-        apply(insert prems9(1,2))[1]
+        apply(insert prems10(1,2))[1]
           apply assumption
-        apply(insert prems9(1,3))
+        apply(insert prems10(1,3))
           apply(rule always_imp_refl)
         done
     apply(rule disjI2)
@@ -97,74 +106,70 @@ apply(erule always_rule)
           apply(erule disjE)
           apply(rule disjI1)
             apply(erule conjE)
-            subgoal premises prems10
-            apply(rule conjI)
-            apply(insert prems10(1,2))[1]
-              apply assumption
-            apply(insert prems10(1,3))
-              apply assumption
-            done
-          apply(rule disjI2)
-            apply(erule conjE)
             subgoal premises prems11
             apply(rule conjI)
             apply(insert prems11(1,2))[1]
               apply assumption
             apply(insert prems11(1,3))
+              apply assumption
+            done
+          apply(rule disjI2)
+            apply(erule conjE)
+            subgoal premises prems12
+            apply(rule conjI)
+            apply(insert prems12(1,2))[1]
+              apply assumption
+            apply(insert prems12(1,3))
               apply(erule conjE)
-              subgoal premises prems12
+              subgoal premises prems13
               apply(rule conjI)
-              apply(insert prems12(1,2))[1]
+              apply(insert prems13(1,2))[1]
                 apply assumption
-              apply(insert prems12(1,3))
+              apply(insert prems13(1,3))
                 apply(erule conjE)
-                subgoal premises prems13
+                subgoal premises prems14
                 apply(rule conjI)
-                apply(insert prems13(1,2))[1]
+                apply(insert prems14(1,2))[1]
                   apply assumption
-                apply(insert prems13(1,3))
+                apply(insert prems14(1,3))
                   apply(erule conjE)
-                  subgoal premises prems14
+                  subgoal premises prems15
                   apply(rule conjI)
-                  apply(insert prems14(1,2))[1]
+                  apply(insert prems15(1,2))[1]
                     apply assumption
-                  apply(insert prems14(1,3))
+                  apply(insert prems15(1,3))
                     apply assumption
                   done
                 done
               done
             done
       apply(rule disjI2)
-        apply(rule since_L7[OF prems1(3)])
-        apply simp
-          apply(erule disjE)
-          apply(rule disjI1)
-            apply(erule conjE)
-            subgoal premises prems15
-            apply(rule conjI)
-            apply(insert prems15(1,2))[1]
-              apply assumption
-            apply(insert prems15(1,3))
-              apply assumption
-            done
-          apply(rule disjI2)
-            apply(erule conjE)
-            subgoal premises prems16
-            apply(rule conjI)
-            apply(insert prems16(1,2))[1]
-              apply assumption
-            apply(insert prems16(1,3))
+        apply(erule disjE)
+        apply(rule disjI1)
+          apply(rule since_L7[OF prems1(3)])
+          apply simp
+            apply(erule disjE)
+            apply(rule disjI1)
+              apply(erule conjE)
+              subgoal premises prems16
+              apply(rule conjI)
+              apply(insert prems16(1,2))[1]
+                apply assumption
+              apply(insert prems16(1,3))
+                apply assumption
+              done
+            apply(rule disjI2)
               apply(erule conjE)
               subgoal premises prems17
               apply(rule conjI)
               apply(insert prems17(1,2))[1]
-                apply(rule always_imp_refl)
+                apply assumption
               apply(insert prems17(1,3))
                 apply(erule conjE)
                 subgoal premises prems18
                 apply(rule conjI)
                 apply(insert prems18(1,2))[1]
-                  apply assumption
+                  apply(rule always_imp_refl)
                 apply(insert prems18(1,3))
                   apply(erule conjE)
                   subgoal premises prems19
@@ -172,11 +177,19 @@ apply(erule always_rule)
                   apply(insert prems19(1,2))[1]
                     apply assumption
                   apply(insert prems19(1,3))
-                    apply assumption
+                    apply(erule conjE)
+                    subgoal premises prems20
+                    apply(rule conjI)
+                    apply(insert prems20(1,2))[1]
+                      apply assumption
+                    apply(insert prems20(1,3))
+                      apply assumption
+                    done
                   done
                 done
               done
-            done
+        apply(rule disjI2)
+          apply assumption
   done
 apply(insert prems3(1,3,5))
   apply(erule previous_rule)
@@ -184,8 +197,8 @@ apply(insert prems3(1,3,5))
   apply(rule impI)
   apply(erule impE)
   apply assumption
-  subgoal premises prems20
-  apply(insert prems20(1,3))
+  subgoal premises prems21
+  apply(insert prems21(1,3))
     apply assumption
   done
 done
@@ -195,43 +208,43 @@ apply(insert prems2(1,3,5))
   apply(rule impI)
   apply(erule impE)
   apply assumption
-  subgoal premises prems21
-  apply(insert prems21(1,3))
+  subgoal premises prems22
+  apply(insert prems22(1,3))
     apply(erule disjE)
     apply(rule disjI1)
-      apply(erule conjE)
-      subgoal premises prems22
-      apply(rule conjI)
-      apply(insert prems22(1,2))[1]
-        apply assumption
-      apply(insert prems22(1,3))
-        apply assumption
-      done
-    apply(rule disjI2)
       apply(erule conjE)
       subgoal premises prems23
       apply(rule conjI)
       apply(insert prems23(1,2))[1]
         apply assumption
       apply(insert prems23(1,3))
+        apply assumption
+      done
+    apply(rule disjI2)
+      apply(erule conjE)
+      subgoal premises prems24
+      apply(rule conjI)
+      apply(insert prems24(1,2))[1]
+        apply assumption
+      apply(insert prems24(1,3))
         apply(erule conjE)
-        subgoal premises prems24
+        subgoal premises prems25
         apply(rule conjI)
-        apply(insert prems24(1,2))[1]
+        apply(insert prems25(1,2))[1]
           apply assumption
-        apply(insert prems24(1,3))
+        apply(insert prems25(1,3))
           apply(erule conjE)
-          subgoal premises prems25
+          subgoal premises prems26
           apply(rule conjI)
-          apply(insert prems25(1,2))[1]
+          apply(insert prems26(1,2))[1]
             apply assumption
-          apply(insert prems25(1,3))
+          apply(insert prems26(1,3))
             apply(erule conjE)
-            subgoal premises prems26
+            subgoal premises prems27
             apply(rule conjI)
-            apply(insert prems26(1,2))[1]
+            apply(insert prems27(1,2))[1]
               apply assumption
-            apply(insert prems26(1,3))
+            apply(insert prems27(1,3))
               apply assumption
             done
           done
@@ -245,43 +258,43 @@ apply(insert prems1(1,3,5))
   apply(rule impI)
   apply(erule impE)
   apply assumption
-  subgoal premises prems27
-  apply(insert prems27(1,3))
+  subgoal premises prems28
+  apply(insert prems28(1,3))
     apply(erule disjE)
     apply(rule disjI1)
-      apply(erule conjE)
-      subgoal premises prems28
-      apply(rule conjI)
-      apply(insert prems28(1,2))[1]
-        apply assumption
-      apply(insert prems28(1,3))
-        apply assumption
-      done
-    apply(rule disjI2)
       apply(erule conjE)
       subgoal premises prems29
       apply(rule conjI)
       apply(insert prems29(1,2))[1]
         apply assumption
       apply(insert prems29(1,3))
+        apply assumption
+      done
+    apply(rule disjI2)
+      apply(erule conjE)
+      subgoal premises prems30
+      apply(rule conjI)
+      apply(insert prems30(1,2))[1]
+        apply assumption
+      apply(insert prems30(1,3))
         apply(erule conjE)
-        subgoal premises prems30
+        subgoal premises prems31
         apply(rule conjI)
-        apply(insert prems30(1,2))[1]
+        apply(insert prems31(1,2))[1]
           apply(rule always_imp_refl)
-        apply(insert prems30(1,3))
+        apply(insert prems31(1,3))
           apply(erule conjE)
-          subgoal premises prems31
+          subgoal premises prems32
           apply(rule conjI)
-          apply(insert prems31(1,2))[1]
+          apply(insert prems32(1,2))[1]
             apply assumption
-          apply(insert prems31(1,3))
+          apply(insert prems32(1,3))
             apply(erule conjE)
-            subgoal premises prems32
+            subgoal premises prems33
             apply(rule conjI)
-            apply(insert prems32(1,2))[1]
+            apply(insert prems33(1,2))[1]
               apply assumption
-            apply(insert prems32(1,3))
+            apply(insert prems33(1,3))
               apply assumption
             done
           done
@@ -291,13 +304,13 @@ apply(insert prems1(1,3,5))
 done
 done
 
-lemma P_2_timeoutseinv_imp_req_gen: "
-P_2_timeouts_inv t1 t2 b_0 b_1 t1_0 b_2 t1_1 A1 A2_1 A3_1 A4_1 s0 \<Longrightarrow>
+lemma P_release_2_timeoutseinv_imp_req_gen: "
+P_release_2_timeouts_inv t1 t2 b_0 b_1 t1_0 b_2 t1_1 A1 A2_1 A3_1 A4_1 A5_1 s0 \<Longrightarrow>
 toEnvP s0 \<Longrightarrow>
-(True \<and> (((always_imp s0 (A3_1 s0) (A3 s0)) \<and> (always_imp s0 (A2_1 s0) (A2 s0))) \<and> ((always_imp s0 (A4_1 s0) (A4 s0)) \<and> True))) \<Longrightarrow>
-P_2_timeouts t1 t2 A1 A2 A3 A4 s0"
+(True \<and> (((always_imp s0 (A3_1 s0) (A3 s0)) \<and> (always_imp s0 (A2_1 s0) (A2 s0))) \<and> (((always_imp s0 (A4_1 s0) (A4 s0)) \<and> True) \<and> (always_imp s0 (\<lambda> r1 . (A5_1 s0 r1)) (\<lambda> r1 . (A5 s0 r1)))))) \<Longrightarrow>
+P_release_2_timeouts t1 t2 A1 A2 A3 A4 A5 s0"
 
-unfolding P_2_timeouts_inv_def P_2_timeouts_def
+unfolding P_release_2_timeouts_inv_def P_release_2_timeouts_def
 subgoal premises prems1
 apply(insert prems1(1,2))
 apply(simp only: conj_assoc)
@@ -333,15 +346,24 @@ apply simp
               apply assumption
             done
         apply(insert prems4(1,3))
-          apply(rule since_L5)
+          apply(rule always_disj_rule)
           apply simp
             apply(erule conjE)
             subgoal premises prems6
             apply(rule conjI)
             apply(insert prems6(1,2))[1]
-              apply assumption
+              apply(rule since_L5)
+              apply simp
+                apply(erule conjE)
+                subgoal premises prems7
+                apply(rule conjI)
+                apply(insert prems7(1,2))[1]
+                  apply assumption
+                apply(insert prems7(1,3))
+                  apply(rule always_imp_refl)
+                done
             apply(insert prems6(1,3))
-              apply(rule always_imp_refl)
+              apply assumption
             done
         done
     done
@@ -349,34 +371,34 @@ done
 done
 done
 
-lemma P_2_timeouts_inv_saving: "
-P_2_timeouts_inv_part t1 t2 b_0 b_1 t1_0 b_2 t1_1 A1 A2 A3 A4 s0 \<Longrightarrow>
+lemma P_release_2_timeouts_inv_saving: "
+P_release_2_timeouts_inv_part t1 t2 b_0 b_1 t1_0 b_2 t1_1 A1 A2 A3 A4 A5 s0 \<Longrightarrow>
 consecutive s0 s \<Longrightarrow>
-(((((b_0 s0) \<or> ((((t1 = 0) \<and> (A2 s)) \<or> ((b_1 s) \<and> ((t1 <= ((t1_0 s0) + 1)) \<and> (A3 s)))) \<or> ((t2 = 0) \<or> ((b_2 s) \<and> ((t2 <= ((t1_1 s0) + 1)) \<and> (A4 s)))))) \<and> ((b_0 s) --> (\<not> (A1 s)))) \<and> ((b_1 s) --> ((((t1_0 s) = 0) \<and> (A2 s)) \<or> ((b_1 s) \<and> (((t1_0 s) <= ((t1_0 s0) + 1)) \<and> (A3 s)))))) \<and> ((b_2 s) --> (((t1_1 s) = 0) \<or> ((b_2 s) \<and> (((t1_1 s) <= ((t1_1 s0) + 1)) \<and> (A4 s)))))) \<Longrightarrow>
-P_2_timeouts_inv_part t1 t2 b_0 b_1 t1_0 b_2 t1_1 A1 A2 A3 A4 s"
+(((((b_0 s0) \<or> ((((t1 = 0) \<and> (A2 s)) \<or> ((b_1 s0) \<and> ((t1 <= ((t1_0 s0) + 1)) \<and> (A3 s)))) \<or> (((t2 = 0) \<or> ((b_2 s0) \<and> ((t2 <= ((t1_1 s0) + 1)) \<and> (A4 s)))) \<or> (A5 s)))) \<and> ((b_0 s) --> (\<not> (A1 s)))) \<and> ((b_1 s) --> ((((t1_0 s) = 0) \<and> (A2 s)) \<or> ((b_1 s0) \<and> (((t1_0 s) <= ((t1_0 s0) + 1)) \<and> (A3 s)))))) \<and> ((b_2 s) --> (((t1_1 s) = 0) \<or> ((b_2 s0) \<and> (((t1_1 s) <= ((t1_1 s0) + 1)) \<and> (A4 s)))))) \<Longrightarrow>
+P_release_2_timeouts_inv_part t1 t2 b_0 b_1 t1_0 b_2 t1_1 A1 A2 A3 A4 A5 s"
 
-unfolding P_2_timeouts_inv_part_def P_2_timeouts_part_def
-apply(simp add: P_2_timeouts_inv_saving_gen always_imp_refl)
+unfolding P_release_2_timeouts_inv_part_def P_release_2_timeouts_part_def
+apply(simp add: P_release_2_timeouts_inv_saving_gen always_imp_refl)
 done
 
-lemma P_2_timeoutseinv_imp_req: "
-P_2_timeouts_inv_part t1 t2 b_0 b_1 t1_0 b_2 t1_1 A1 A2 A3 A4 s \<Longrightarrow>
+lemma P_release_2_timeoutseinv_imp_req: "
+P_release_2_timeouts_inv_part t1 t2 b_0 b_1 t1_0 b_2 t1_1 A1 A2 A3 A4 A5 s \<Longrightarrow>
 toEnvP s \<Longrightarrow>
 True \<Longrightarrow>
-P_2_timeouts_part t1 t2 A1 A2 A3 A4 s"
+P_release_2_timeouts_part t1 t2 A1 A2 A3 A4 A5 s"
 
-unfolding P_2_timeouts_inv_part_def P_2_timeouts_part_def
-apply(simp add: P_2_timeoutseinv_imp_req_gen always_imp_refl)
+unfolding P_release_2_timeouts_inv_part_def P_release_2_timeouts_part_def
+apply(simp add: P_release_2_timeoutseinv_imp_req_gen always_imp_refl)
 done
 
 
 
-lemmas P_2_timeouts_used_patterns = P_2_timeouts_def always_used_patterns weak_previous_def since_def since_def 
+lemmas P_release_2_timeouts_used_patterns = P_release_2_timeouts_def always_used_patterns weak_previous_def since_def since_def 
 
-lemmas P_2_timeouts_inv_used_patterns = P_2_timeouts_inv_def always_inv_used_patterns weak_previous_def since_def since_def previous_inv_def since_inv_def since_inv_def 
+lemmas P_release_2_timeouts_inv_used_patterns = P_release_2_timeouts_inv_def always_inv_used_patterns weak_previous_def since_def since_def previous_inv_def since_inv_def since_inv_def 
 
-lemmas P_2_timeouts_inv_part_used_patterns = P_2_timeouts_inv_part_def P_2_timeouts_inv_used_patterns
+lemmas P_release_2_timeouts_inv_part_used_patterns = P_release_2_timeouts_inv_part_def P_release_2_timeouts_inv_used_patterns
 
-lemmas P_2_timeouts_part_used_patterns = P_2_timeouts_part_def P_2_timeouts_used_patterns
+lemmas P_release_2_timeouts_part_used_patterns = P_release_2_timeouts_part_def P_release_2_timeouts_used_patterns
 
 end
